Some renames

test/test.lean
@@ -1,22 +1,24 @@
-import config
+import iconfig
 
-open config
+section
 
 iconfig_mk my_tac
 
 iconfig_add my_tac [
-  abool  : config.boolc {},
-  anum   : config.nat,
-  aenum  : config.enat,
-  astr   : config.string,
-  aident : config.ident,
+  abool  : iconfig.boolc {},
+  anum   : iconfig.nat,
+  aenum  : iconfig.enat,
+  astr   : iconfig.string,
+  aident : iconfig.ident,
 ]
+
+end
 
 namespace tactic
 namespace interactive
 
 meta def cfgdump (c : iconfig my_tac) : tactic unit := do
-  l ← config.read c,
+  l ← iconfig.read c,
   l.bool "abool" >>= tactic.trace,
   return ()
 
@@ -24,13 +26,13 @@ end interactive
 end tactic
 
 example : tt := begin
-  cfgdump begin
+  cfgdump {
     abool := ff,
     anum := 113,
     aenum := inf,
     astr := "ello",
     aident s.sss4,
-  end,
+  },
 
   simp
 end
