src/iconfig/monad.lean
@@ -1,0 +1,30 @@
+import .cfgopt
+
+meta def iconfig_tac (α : Type) :=
+tactic α
+
+meta instance : monad iconfig_tac :=
+by dunfold iconfig_tac; apply_instance
+
+meta instance : monad_fail iconfig_tac :=
+by dunfold iconfig_tac; apply_instance
+
+meta instance : alternative iconfig_tac :=
+by dunfold iconfig_tac; apply_instance
+
+namespace iconfig
+
+meta def save_info (p : pos) : iconfig_tac unit :=
+do s ← tactic.read,
+   tactic.save_info_thunk p (λ _, s.to_format tt)
+
+meta def step {α : Type} (c : iconfig_tac α) : iconfig_tac unit :=
+c >> return ()
+
+meta def istep {α : Type} (line0 col0 line col : _root_.nat) (c : iconfig_tac α) : iconfig_tac unit :=
+tactic.istep line0 col0 line col c
+
+meta def execute (c : iconfig_tac unit) : tactic unit :=
+c
+
+end iconfig
